\documentclass{article}
\usepackage[utf8]{inputenc}
\usepackage{amsmath}
\usepackage{parskip}
\usepackage{dsfont}
\usepackage{fullpage}

\title{Riemann Hypothesis}
\author{Paolo Bettelini}
\date{June 2021}

\begin{document}

\maketitle
\tableofcontents
\pagebreak

\section{Zeta function}

\subsection{Definition}

The zeta function is defined as

\begin{align*}
    \zeta(s)=\sum_{n=1}^{\infty}\frac{1}{n^s},\quad Re(s)>0
\end{align*}

\subsection{Euler product}

The zeta function can be represented as an Euler product.
\\
We will start by using the first prime number: 2.

\begin{align*}
    \zeta(s)\frac{1}{2^s}=\sum_{n=1}^{\infty}\frac{1}{(2n)^s}
\end{align*}

We then subtract the second definition from the first one, such that

\begin{align*}
    \begin{split}
        \zeta(s)-\zeta(s)\frac{1}{2^s}&=
        \sum_{n=1}^{\infty}\left[\frac{1}{n^s}\right]-
        \sum_{n=1}^{\infty}\left[\frac{1}{(2n)^s}\right]
        \\
        \zeta(s)\left(1-\frac{1}{2^s}\right)&=
        \sum_{n=1}^{\infty}\frac{1}{n^s},
        \quad n\neq 2k,k\in \mathds{Z}
    \end{split}
\end{align*}

Here we are excluding the multiples of 2 from the series.

If we do the same with the next prime number, which is 3, we get

\begin{align*}
    \zeta(s)\left(1-\frac{1}{2^s}\right)\left(1-\frac{1}{3^s}\right)&=
    \sum_{n=1}^{\infty}\frac{1}{n^s},
    \quad n\neq 2k_1,n\neq 3k_2, k\in \mathds{Z}
\end{align*}

We can repeat this process with every prime number.
\\
Eventually, we will exclude every nth-term to sum as we use every prime number, except for n=1.

\begin{align*}
    \zeta(s)\prod_{p\in P}^{\infty}1-\frac{1}{p^s}=\frac{1}{1^s}=1
\end{align*}

Finally, we get the identity

\begin{align*}
    \zeta(s)=
    \prod_{p\in P}^{\infty}\frac{1}{1-p^{-s}}
\end{align*}

\pagebreak

\section{Prime-counting function}

\subsection{Properties of the prime-counting function}

The prime-counting function $\pi (x)$ is defined as the number of primes less or equals than $x$.

We can consider the difference between $\pi (x)$ of two consecutive integers
\begin{align*}
    \pi (x)-\pi (x-1)= 
    \begin{cases}
        1,& \text{if } x\in P
        \\
        0,& \text{otherwise}
    \end{cases}
\end{align*}

Given a series over all prime numbers, we can extend it to all integers and multiply each term by this difference.
\\
The terms whose index is not a prime number will be multiplied by 0.

\begin{align*}
    \sum_{p\in P}^{\infty}a_k=\sum_{n=2}^{\infty}\left[\pi (n) - \pi (n-1)\right]a_n
\end{align*}

Here we start at 2 since there are no prime numbers less than 2.

\subsection{Relationship with the zeta function}

We have seen that the zeta function can be written as an Euler Product

\begin{align*}
    \zeta (s)=\prod_{p\in P}^{\infty}\frac{1}{1-p^{-s}}
\end{align*}

However, we need convert this product into a series in order to apply the identity of the last paragraph.
\\
We can take the natural logarithm of both sides and use the multiplication property

\begin{align*}
    \begin{split}
        ln\left(\zeta (s)\right)&=ln\prod_{p\in P}^{\infty}\frac{1}{1-p^{-s}}
        \\
        &=\sum_{p\in P}^{\infty}ln\left(\frac{1}{1-p^{-s}}\right)
        \\
        &=\sum_{p\in P}^{\infty}-ln\left(1-p^{-s}\right)
    \end{split}
\end{align*}

Now we can apply the identity

\begin{align*}
    ln\left(\zeta (s)\right)=\sum_{n=2}^{\infty}-ln\left(1-n^{-s}\right)\left[\pi (n) - \pi (n-1)\right]
\end{align*}

The next goal is to factor out $\pi (n)$

\begin{align*}
    \begin{split}
        ln\left(\zeta (s)\right)&=\sum_{n=2}^{\infty}\left[\pi (n-1)ln\left(1-n^{-s}\right)\right]
        -\sum_{n=2}^{\infty}\left[\pi (n)ln\left(1-n^{-s}\right)\right]
        \\&=\sum_{n=2}^{\infty}\left[\pi (n)ln\left(1-(n+1)^{-s}\right)\right]
        -\sum_{n=2}^{\infty}\left[\pi (n)ln\left(1-n^{-s}\right)\right]
        \\
        &=\sum_{n=2}^{\infty}\pi (n)\left[ln\left(1-(n+1)^{-s}\right)-ln\left(1-n^{-s}\right)\right]
    \end{split}
\end{align*}

[...]

\end{document}