\documentclass[preview]{standalone}

\usepackage{amsmath}
\usepackage{amssymb}
\usepackage{stellar}
\usepackage{definitions}
\usepackage{bettelini}

\begin{document}

\id{settheory-basic-results}
\genpage

\section{Basic results}

\begin{snippetcorollary}{subset-of-itself}{Every set is subset of itself}
    For every \set \(A\), \(A \subseteq A\).
\end{snippetcorollary}

\begin{snippettheorem}{vacuous-truth-theorem}{Vacuous truth}
    For any proposition \(P(n)\), if the domain of discourse for \(x\) is \(\emptyset\), then
    \[\forall x\in\emptyset, P(x) \]
\end{snippettheorem}

\begin{snippetcorollary}{empty-set-is-subset-of-any-set}{Empty set is subset of any set}
    For every \set \(A\),
    \(\emptyset \subseteq A\).
\end{snippetcorollary}

\begin{snippetcorollary}{subset-of-powerset}{Subset of powerset}
    For every \set \(B\), \(B\in\powerset(B)\).
\end{snippetcorollary}

\begin{snippetcorollary}{set-equivalence-with-subsets}{Set equivalence with subsets}
    Let \(A\) and \(B\) be \set[sets].
    \[ A = B \iff A \subseteq B \land B \subseteq A \]
\end{snippetcorollary}

\begin{snippetcorollary}{subseteq-transitivity}{Subset transitivity}
    Let \(A\), \(B\) and \(C\) be \set[sets].
    \begin{align*}
        &1. \quad A \subseteq B \land B \subseteq C \implies A \subseteq C \\
        &2. \quad A \subset B \land B \subseteq C \implies A \subset C \\
        &3. \quad A \subseteq B \land B \subset C \implies A \subset C \\
        &4. \quad A \subset B \land B \subset C \implies A \subset C
    \end{align*}
\end{snippetcorollary}

\begin{snippetproof}{subseteq-transitivity-proof}{subseteq-transitivity}{Subset transitivity}
    Without loss of generality (1) we have \(B \subseteq C \implies \forall b \in B, b \in C\)
    and \(A \subseteq B \implies \forall a \in A, a \in B\).
    This implies that \(\forall a \in A, a \in C\) and thus \(A \subseteq C\).
\end{snippetproof}

\begin{snippetproposition}{proper-subsets-with-subsets}{Proper subsets with subsets}
    Let \(A\) and \(B\) be \set[sets].
    \[ A \subset B \iff A \subseteq B \land B \notsubseteq A \]
\end{snippetproposition}

\begin{snippetproposition}{dual-set-difference}{Dual set difference}
    Let \(A\) and \(B\) be \set[sets].
    \[
        A \difference B = B \difference A
        \iff A = B
    \]
\end{snippetproposition}

\begin{snippetproof}{dual-set-difference-proof}{dual-set-difference}{Dual set difference}
    \iffproof{
        \begin{itemize}
            \item \(\mathbf{A \subseteq B}\): let \(x\in B\). If \(x\notin A\), then \(x \in B \difference A\). Since \(A \difference B = B \difference A\),
            we have that \(x \in A \difference B\), which implies \(x\in A\) and \(x\notin B\), which is absurd \lightning.
            Therefore, if \(x\in A\), then \(x\in B\). Thus, \(A \subseteq B\).
            \item \(\mathbf{B \subseteq A}\): let \(x\in A\). If \(x\notin B\), then \(x \in A \difference B\). Since \(A \difference B = B \difference A\),
            we have that \(x \in B \difference A\), which implies \(x\in B\) and \(x\notin A\), which is absurd \lightning.
            Therefore, if \(x\in B\), then \(x\in A\). Thus, \(B \subseteq A\).
        \end{itemize}
        Since \(B \subseteq A \land A \subseteq B\), we have that \(A=B\).
    }{
        Since \(A = B\), we have that \(A \difference B = B \difference A = \emptyset\).
    }
\end{snippetproof}

\begin{snippetcorollary}{subset-in-terms-of-relationships}{Subset in terms of relationships}
    \[
        A \subseteq B
        \iff
        A \union B = B
        \iff
        A \intersection B = A
        \iff
        A \difference B = \emptyset
    \]
\end{snippetcorollary}

\begin{snippetproof}{subset-in-terms-of-relationships-proof}{subset-in-terms-of-relationships}{Subset in terms of relationships}
    We prove various propositions to prove the equivalence
    \begin{itemize}
        \item \(a \subseteq B \implies A \union B = B\):
            assume \(a \subseteq B\). We must show that \(A \union B \subseteq B \land A \union B \supseteq B\).
            The second piece is trivially true without assumptions. For the \(A \union B \subseteq B\) part,
            let \(x\in A \union B\). We know that \(x\in A \lor x\in B\). In the first caso, we have \(x\in B\),
            while the second cse is already what we want.
            \item \(A \union B = B \implies A \intersection B = A\): \todo
            \item \(A \intersection B = A \implies A \difference B = \emptyset\): \todo
            \item \(A \difference B = \emptyset \implies A \subseteq B\): \todo
    \end{itemize}
\end{snippetproof}

\begin{snippetproposition}{set-equivalence-power-set-equivalence}{Set and power set equivalence}
    Let \(A\) and \(B\) be \set[sets].
    \[ A = B \iff \powerset(A) = \powerset(B) \]
\end{snippetproposition}

\begin{snippetproof}{set-equivalence-power-set-equivalence-proof}{set-equivalence-power-set-equivalence}{Set and power set equivalence}
    \iffproof{
        Assume \(A=B\), then \(\powerset(A) = \powerset(B)\).
    }{
        Assume \(\powerset(A) = \powerset(B)\),
        \(A \in \powerset(A)\) and \(A \in \powerset(B)\), and thus \(A \subseteq B\).
        Likewise, we can show that \(B \subseteq A\), and by
        \snippetref[set-equivalence-with-subsets][set equivalence with subsets] we have \(A=B\).
    }
\end{snippetproof}

\begin{snippettheorem}{cardinality-of-the-power-set}{Cardinality of the power set}
    Let \(A\) be a \set where \(\cardinality{A} < \infty\). The cardinality of \(\powerset(A)\) is given by
    \[
        \cardinality{\powerset(A)} = 2^{\cardinality{A}}
    \]
\end{snippettheorem}

\begin{snippetproof}{cardinality-of-the-power-set-proof}{cardinality-of-the-power-set}{Cardinality of the power set}
    Let \(A\) be a \set where \(\cardinality{A} < \infty\).
    To find \(\cardinality{\powerset(A)}\) we can count all the ways of selecting
    \(k\) out of \(n=\cardinality{S}\) elements with \(k=0,1,\cdots, n\).
    \[
        \cardinality{\powerset(A)} = \sum_{k=0}^n \binom{n}{k}
    \]
    From the \snippetref[binomial-theorem][binomial theorem] we have that
    \[
        \cardinality{\powerset(A)} = \sum_{k=0}^n \binom{n}{k} 1^{n-k}1^k = {(1+1)}^n = 2^n
    \]
\end{snippetproof}

\begin{snippetcorollary}{infinite-set-power-set-is-infinite}{Power set of infinite set is infinite}
    Let \(A\) be a \set where \(\cardinality{A} = \infty\).
    \[ \cardinality{\powerset(A)} =\infty \]
\end{snippetcorollary}

\begin{snippetproof}{infinite-set-power-set-is-infinite-proof}{infinite-set-power-set-is-infinite}{Power set of infinite set is infinite}
    Let \(A\) be a \set where \(\cardinality{A} = \infty\).
    Let's assume that \(\cardinality{\powerset(A)} < \infty\), then there would be a finite number of subsets of \(A\).
    This implies that there is only a maximum numbers of distinct subsets that can be formed from \(A\),
    but an infinite set should always be able to create an infinite amount of distinct subsets \lightning.
\end{snippetproof}

\begin{snippetproposition}{set-union-intersection-commutative}{Union and intersection are commutative}
    Let \(A\) and \(B\) be \set[sets]. Then:
    \begin{enumerate}
        \item \(A \union B = B \union A\);
        \item \(A \intersection B = B \intersection A\).
    \end{enumerate}
\end{snippetproposition}

\begin{snippetproof}{set-union-intersection-commutative-proof}{set-union-intersection-commutative}{Union and intersection are commutative}
    \begin{enumerate}
        \item Let \(x\in A \union B\). This means that \(x \in A \lor x \in B\), which is the same as \(x \in B \lor x \in A\),
        which is the definition of \(x \in B \union A\);
        \item Let \(x\in A \intersection B\). This means that \(x \in A \land x \in B\), which is the same as \(x \in B \land x \in A\),
        which is the definition of \(x \in B \intersection A\);
    \end{enumerate}
\end{snippetproof}

\begin{snippetproposition}{set-union-intersection-associative}{Union and intersection are associative}
    Let \(A\), \(B\) and \(C\) be \set[sets]. Then:
    \begin{enumerate}
        \item \((A \union B) \union C = A \union (B \union C)\);
        \item \((A \intersection B) \intersection C = A \intersection (B \intersection C)\).
    \end{enumerate}
    Thus, parenthesis are therefore not needed.
\end{snippetproposition}

\begin{snippetproof}{set-union-intersection-associative-proof}{set-union-intersection-associative}{Union and intersection are associative}
    \begin{enumerate}
        \item Let \(x\in (A \union B) \union C\). By definition, this means that \((x\in A \lor x\in B) \lor x\in C\).
        However, this is equivalent to \(x\in A \lor (x\in B \lor x\in C)\), which is the definition of \(A \union (B \union C)\);
        \item Let \(x\in (A \intersection B) \intersection C\). By definition, this means that \((x\in A \land x\in B) \land x\in C\).
        However, this is equivalent to \(x\in A \land (x\in B \land x\in C)\), which is the definition of \(A \intersection (B \intersection C)\).
    \end{enumerate}
\end{snippetproof}

\begin{snippetproposition}{subset-relation-union-intersection}{Subset relations in union and intersection}
    Let \(A\), \(B\) and \(C\) be \set[sets].
    \begin{enumerate}
        \item \(A \subseteq A \union B\);
        \item \(A \supseteq A \intersection B\);
        \item \(B \subseteq A \union B\);
        \item \(B \supseteq A \intersection B\).
    \end{enumerate}
\end{snippetproposition}

\begin{snippetproof}{subset-relation-union-intersection-proof}{subset-relation-union-intersection}{Subset relations in union and intersection}
    \begin{enumerate}
        \item Let \(x\in A\). Then \(x \in A \lor x \in B\), which is the definition of \(A \union B\). Thus, \(A \subseteq A \union B\).
        \item Let \(x\in A \intersection B\). Then, \(x \in A \land x \in B\). In particular, \(x \in A\). Thus, \(A \intersection B \subseteq A\).
        \item Let \(x\in B\). Then \(x \in B \lor x \in A\), which is the definition of \(A \union B\). Thus, \(B \subseteq A \union B\).
        \item Let \(x\in A \intersection B\). Then, \(x \in A \land x \in B\). In particular, \(x \in B\). Thus, \(A \intersection B \subseteq B\).
    \end{enumerate}
\end{snippetproof}

\begin{snippetproposition}{set-distributivity-intersection-over-union}{Distributivity of Intersection over Union}
    Let \(A\), \(B\) and \(C\) be \set[sets].
    \[ A \intersection (B \union C) = (A \intersection B) \union (A \intersection C) \]
\end{snippetproposition}

\begin{snippetproof}{set-distributivity-intersection-over-union-proof}{set-distributivity-intersection-over-union}{Distributivity of Intersection over Union}
    We first show that \(A \intersection (A \union C) \subseteq (A \intersection B) \union (A \intersection C)\).
    Let \(x\in A \intersection (B \union C)\), we must show that \(x\in (A \intersection B) \union (A \intersection C)\).
    We know that \(x\in A\) and \(x\in B \union C\), which tells us that
    at least one of \(x\in B\) or \(x\in C\) is true.
    Consider the case where \(x\in B\). Since \(x\in A\), we have that \(x\in A \intersection B\)
    and thus \(x\in (A \intersection B) \union (A \intersection C)\).
    Likewise, if \(x\in C\), we have that \(x\in A \intersection C\), and thus \(x\in A \intersection C\).
    We now show that \(A \intersection (B \union C) \supseteq (A \intersection B) \union (A \intersection C)\).
    Let \(x\in (A \intersection B) \union (A \intersection C)\), which means that
    \(x \in A \intersection B \lor x \in A \intersection C\).
    In the first case, \(x \in A \land x\in B\), and from the second \(x\in B \union C\).
    Since \(x\in A\), we have \(x \in A \intersection (B \union C)\).
    The same goes for \(x\in A \intersection C\).
\end{snippetproof}

\begin{snippetproposition}{set-distributivity-union-over-intersection}{Distributivity of Union over Intersection}
    Let \(A\), \(B\) and \(C\) be \set[sets].
    \[ A \union (B \intersection C) = (A \union B) \intersection (A \union C) \]
\end{snippetproposition}

% TODO proof

\begin{snippetproposition}{subset-characterization-union-and-intersection}{}
    Let \(A\), \(B\) and \(C\) be \set[sets].
    \begin{enumerate}
        \item \(A \union B \subseteq C \iff A \subseteq C \land B \subseteq C\);
        \item \(A \intersection B \supseteq C \iff A \supseteq C \land B \supseteq C\).
    \end{enumerate}
\end{snippetproposition}

\end{document}