\documentclass[preview]{standalone}

\usepackage{amsmath}
\usepackage{amssymb}
\usepackage{stellar}
\usepackage{definitions}
\usepackage{bettelini}

\begin{document}

\id{rings-introduction}
\genpage

\section{Definition}

\begin{snippetdefinition}{ring-definition}{Ring}
    A \textit{ring} \((R, +, \circ)\) is a triple containing a \set \(R\) and two \binoperation[binary operations]
    \(+\) and \(\circ\) on \(R\) such that:
    \begin{enumerate}
        \item \((R, +)\) is an \abeliangroup;
        \item \((R, \circ)\) is a \monoid;
        \item \textit{left distributivity}: \(\forall a,b,c\in R, a\circ(b+c) = (a\circ b) + (a \circ c)\);
        \item \textit{right distributivity}: \(\forall a,b,c\in R, (b+c)\circ a = (b\circ a) + (c \circ a)\).
    \end{enumerate}
\end{snippetdefinition}

\begin{snippetdefinition}{commutative-ring-definition}{Commutative ring}
    A \ring \((R, +, \circ)\) is said to be \textit{commutative} if:
    \begin{enumerate}
        \item \textit{distributivity}: \(\forall a,b\in R, a\circ b = b\circ a\).
    \end{enumerate}
\end{snippetdefinition}

\begin{snippetproposition}{ring-zero-multiplication}{}
    Let \(A = (R, +, \circ)\) be a \ring. Then, \[
        a \circ 0_A = 0_A, \quad \forall a \in R
    \]
\end{snippetproposition}

\begin{snippetproof}{ring-zero-multiplication-proof}{ring-zero-multiplication}{}
    We first note that \(0_A = 0_A + 0_A\)
    and that \(0_A \circ a = a \circ 0_A = 0_A\).
    From this we get \(a \circ 0_A = a \circ 0_A + a \circ 0_A\)
    and by subtracting we get \(0_A \circ a = 0_A\).
    Likewise, we find that \(a \circ 0_A = 0_A\).
\end{snippetproof}

\begin{snippetproposition}{ring-inverse-addition-multiplication}{}
    Let \(A = (R, +, \circ)\) be a \ring. Then, \[
        - a = (- 1_A) \circ a = a \circ (- 1_A), \quad \forall a \in R
    \]
\end{snippetproposition}

\begin{snippetproof}{ring-inverse-addition-multiplication-proof}{ring-inverse-addition-multiplication}{}
    We have
    \begin{align*}
        1_A + (-1_A) &= 0_A \\
        0_A &= a \circ 0_A = a \circ (1_A + (1_A)) = a \circ 1_A + a \circ (-1_A) \\
        &= a + a \circ (-1_A) \\
        -a &= a \circ (-1_A)
    \end{align*}
    Likewise, we find \(-a = (-1_A) \circ a\).
\end{snippetproof}

\plain{We can define the multiplication by an integer as repeated addition.}

\begin{snippetproposition}{ring-multiplication-as-addition}{}
    Let \(A = (R, +, \circ)\) be a \ring. Then, \[
        n(ab) = (ab)n = a(nb)
    \]
    and
    \[
        (-n) \circ a = -(n \circ a)
    \]
\end{snippetproposition}

\begin{snippetproof}{ring-multiplication-as-addition-proof}{ring-multiplication-as-addition}{}
    By induction:
    \begin{enumerate}
        \item the base case is \(n=2\),
        \[
            2(ab) = ab + ab = \begin{cases}
                a(b+b) = a(2b) \\
                (a+a)b = (2a)b
            \end{cases}
        \]
    \end{enumerate}
\end{snippetproof}

\plain{Using these properties we can prove prove that a negative times a negative is a positive.}

\begin{snippetdefinition}{ring-zero-divisor-definition}{Zero divisor}
    Let \(A = (R, +, \circ)\) be a \ring and \(a \in R\) such that \(a \neq 0_A\).
    We say that \(a\) is a \emph{left or right zero divisor} if
    \[
        \exists b \in R \suchthat b \neq 0_A \land a \circ b = 0_A
    \]
    or
    \[
        \exists b \in R \suchthat b \neq 0_A \land b \circ a = 0_A
    \]
    respectively.
\end{snippetdefinition}

\begin{snippetdefinition}{integral-domain-definition}{Integral domain}
    Let \(A = (R, +, \circ)\) be a commutative \ring.
    Then, \(A\) is said to be an \emph{integral domain}
    if it does not contain any zero divisor.
\end{snippetdefinition}

\begin{snippetproposition}{zero-divisors-are-not-invertible}{Zero divisors are not invertible}
    Let \(A = (R, +, \circ)\) be a \ring and \(a \in R\)
    a zero divisor. Then, \(a\) is not invertible.
\end{snippetproposition}

\begin{snippetproof}{zero-divisors-are-not-invertible-proof}{zero-divisors-are-not-invertible}{zero divisors are not invertible}
    There exist a non-null \(b \in R\) such that \(ab = 0_A\).
    Suppose that \(a^{-1} \in A\). We then have
    \begin{align*}
        a^{-1} \circ a \circ b &= 1_A \circ b = b = 0_A \circ a^{-1} = 0_A
    \end{align*}
    which is absurd \lightning.
\end{snippetproof}

\begin{snippetproposition}{zero-divisors-simplification}{}
    Let \(A = (R, +, \circ)\) be a \ring and \(a \in R\)
    such that \(a\neq 0_A\) is not a left/right zero-divisor. Then,
    \[
        a \circ b = a \circ c \implies b = c
    \]
    and
    \[
        b \circ a = c \circ a \implies b = c
    \]
    respectively.
\end{snippetproposition}

\begin{snippetproof}{zero-divisors-simplification-proof}{zero-divisors-simplification}{}
    We will prove the left case
    \begin{align*}
        ab &= ac \\
        ab + (-ac) &= 0_A \\
        a\circ (b-c) &= 0_A
    \end{align*}
    Since there are no zero-divisors, either \(a\) or \(b-c\) is null.
    Since \(a \neq 0\), \(b-c = 0_A\).
\end{snippetproof}

\begin{snippetdefinition}{subring-definition}{Subring}
    Let \(A = (R, +, \circ)\) be a \ring.
    A \emph{subring} of \(A\) is a subset \(S \subseteq R\)
    such that \((S, +, \circ)\) is a \ring.
\end{snippetdefinition}

\begin{snippetdefinition}{ring-ideal-definition}{Ideal}
    Let \(A = (R, +, \circ)\) be a \ring.
    A \emph{left/right ideal} of \(A\) is a subset \(I \subseteq R\)
    such that:
    \begin{enumerate}
        \item \((I, +)\) is a \subgroup of \((R, +)\);
        \item \(\forall i \in I, \forall r \in R\), we have \(ir \in I\) (left ideal) and \(ri \in I\) (right ideal).
    \end{enumerate}
    If the ideal is both a left and right ideal, it is called a
    \emph{two-sided ideal}, \emph{bilateral} or simply an \emph{ideal}.
\end{snippetdefinition}

\plain{In a commutative ring, every ideal is bilateral.}

\begin{snippetproposition}{ring-ideal-identity}{}
    Let \(A\) be a \ring and \(I \idealin A\) such that \(1_A \in I\).
    Then, \(A = I\).
\end{snippetproposition}

\begin{snippetproof}{ring-ideal-identity-proof}{ring-ideal-identity}{}
    We have:
    \begin{enumerate}
        \item if the ideal is left, \(\forall a \in A, a = 1_A \cdot a \in I\) and thus \(A \subseteq I\);
        \item if the ideal is right, \(\forall a \in A, a = a \cdot 1_A \in I\) and thus \(A \subseteq I\).
    \end{enumerate}
\end{snippetproof}

\begin{snippetproposition}{trivial-ring-ideals}{}
    Let \(A\) be a \ring.
    Then, \(A, \{0_A\} \idealin A\).
\end{snippetproposition}

\begin{snippetproposition}{ring-subsets-intersection}{}
    Let \(A\) be a \ring and \(\{B_i\}_{i \in I} \leq A\).
    Then,
    \[
        B = \left(\bigcap_{i \in I} B_i\right) \leq A
    \]
\end{snippetproposition}

\begin{snippetproof}{ring-subsets-intersection}{ring-subsets-intersection}{}
    We have \(0_A, 1_A \in B\).
    For all \(a,b \in B, a,b \in B_i\) for all \(i \in I\).
\end{snippetproof}

\plain{This does not work in general for the sum and union.}

\begin{snippetdefinition}{algebra-definition}{Algebra}
    Let \(\mathbb{F}\) be a \field and \(A\) a \set and let
    \begin{align*}
        + \colon A \cartesianprod A \fromto A \\
        \circ \colon A \cartesianprod A \fromto A \\
        \cdot \colon F \cartesianprod A \fromto A
    \end{align*}
    Then, \(A\) is a \emph{\(\mathbb{F}\)-algebra} if:
    \begin{enumerate}
        \item \((A, +, \circ)\) is a \ring;
        \item \((A, +, \cdot)\) is a \vectorspace over \(\mathbb{F}\);
        \item \(\forall a,b \in A, \forall \lambda \in \mathbb{F}, (\lambda \cdot a) \circ b = \lambda \cdot (a\circ b)\).
    \end{enumerate}
\end{snippetdefinition}

\begin{snippet}{algebra-as-subring}
    Let \(\mathbb{F}\) be a \field and \(A\) a \ring.
    Then, in the \algebra induced by \(A\)
    we can see the field as a subring
    \[
        \{\lambda \cdot 1_A \suchthat \lambda \in \mathbb{F}\} \leq A
    \]
\end{snippet}

\begin{snippetexample}{algebra-example1}{}
    Let \(\mathbb{K}\) be a \field.
    Then, \(\mathbb{K}[x]\) is an \algebra over \(\mathbb{K}\)
    \[
        \{\lambda \cdot 1\}
    \]
\end{snippetexample}

\begin{snippetdefinition}{multiplicative-group-of-ring-definition}{Multiplicative group}
    The \emph{multiplicative} group of a \ring \(A\)
    is the \group
    \[
        A^x = \{
            a \in A \suchthat a^{-1} \in A    
        \}
    \]
\end{snippetdefinition}

\subsection{Morphisms}

\begin{snippetdefinition}{ring-homomorphism-definition}{Ring homomorphism}
    Let \((A, \cdot, +)\) and \((H, \circ, \ast)\) be \ring[rings].
    A \function \(\varphi\colon A \fromto B\)
    such that:
    \begin{enumerate}
        \item it is a \grouphomomorphism;
        \item \(\varphi(1_A) = 1_B\)
        \item \emph{morphism property:} \(\forall a_1,a_2 \in A, \varphi(a_1\cdot a_2) = \varphi(a_1) \circ \varphi(a_2)\)
    \end{enumerate}
    is said to be a \emph{ring homomorphism}.
\end{snippetdefinition}

\begin{snippetdefinition}{ring-kernel-definition}{Ring kernel}
    \todo
    % pure il kernel che manca in 0_B
\end{snippetdefinition}

\begin{snippetproposition}{ring-homomorphism-properties}{}
    Let \(\varphi \colon A \fromto B\) be a \ringhomomorphism. Then,
    \begin{enumerate}
        \item if \(a \in A^x\), then \(\varphi(x) \in B^x\);
        \item if \(S \leq A\), then \(\varphi(S) \leq B\);
        \item if \(R \leq B\), then \(\varphi^{-1}(R) = \{a \in A \suchthat \varphi(a) \in R\} \leq A\);
        \item \(\ringker_\varphi \idealin A\);
        \item \(\varphi\) is \injective \ifandonlyif \(\ringker_\varphi = \{0_A\}\).
    \end{enumerate}
\end{snippetproposition}

\begin{snippetproof}{ring-homomorphism-properties-proof}{ring-homomorphism-properties}{}
    \begin{enumerate}
        \item there exist \(b\in A\) such that \(ab = 1_A\), meaning
        \[
            \varphi(a) \cdot \varphi(b) = \varphi(ab) = \varphi(1_A) = 1_B
        \]
        \item \begin{enumerate}
            \item \(\varphi(S)\) è closed under addition and multiplication and \(0_B, 1_B \in \varphi(S)\);
            \item \(0_A \in S \implies 0_B = \varphi(0_A) \in \varphi(S)\)
            and \(1_A \in S \implies 1_B = \varphi(1_A) \in \varphi(S)\).
            \item if \(b_1, b_2 \in \varphi(S)\) there exist \(a_1, a_2 \in S\)
            such that \(\varphi(a_i) = b_i\) for \(i=1,2\).
            This means that
            \begin{align*}
                b_1 - b_2 &= \varphi(a_1) - \varphi(a_2) = \varphi(a_1 - a_2) \in \varphi(S) \\
                b1 \cdot b_2 &= \varphi(b_1) \cdot \varphi(b_2) = \varphi(b_1 \cdot b_2) \in \varphi(S)
            \end{align*}
            \item we have \(1_A \in \varphi^\inversefunction(1_B)\)
            and \(0_A \in \varphi^\inversefunction(0_B)\).
            If \(a_1, a_2 \in \varphi^\inversefunction(R)\) we have
            \(\varphi(a_1),\varphi(a_2) \in R\) and thus
            \begin{align*}
                \varphi(a_1) - \varphi(a_2) &= \varphi(a_1 - a_2) \\
                \varphi(a_1) \cdot \varphi(a_2) = \varphi(a_1 \cdot a_2)
            \end{align*}
            which meman \(a_1 - a_2\in \varphi^\inversefunction(R)\)
            and \(a_1 \cdot a_2\in \varphi^\inversefunction(R)\).
            \item It is clear that \(0_A \in \ringker_\varphi\)
            and that if \(x,y \in \ringker_\varphi\) then \(x-y \in \ringker_\varphi\).
            For all \(x \in \ringker_\varphi\) and for all \(a \in A\),
            \begin{align*}
                \varphi(ax) &= \varphi(a) \cdot \varphi(x)
                = \varphi(a) \cdot 0_B = 0_B \\
                \varphi(xa) = \varphi(x) \cdot \varphi(a) = 0_B \cdot \varphi(a) = 0_B
            \end{align*}
            it is thus a \ideal[bilateral ideal].
            \item \iffproof{
                If \(\varphi\) is \injective,
                \(\varphi(0_A) = 0_B\) which means that \(\ringker_\varphi = \{0_A\}\).
            }{
                If \(\ringker_\varphi = \{0_A\}\), \(\forall a_1, a_2 \in A\) we have
                \[
                    \varphi(a_1) - \varphi(a_2) = \varphi(a_1 - a_2)
                \]
                But if \(\varphi(a_1) = \varphi(a_2)\), then
                \(a_1 - a_2 \in \ringker_\varphi = \{0_A\}\)
                and thus \(a_1 = a_2\).
            }
        \end{enumerate}
    \end{enumerate}
\end{snippetproof}

\end{document}