\documentclass[preview]{standalone}

\usepackage{amsmath}
\usepackage{amssymb}
\usepackage{stellar}
\usepackage{definitions}

\begin{document}

\id{asymptotes}
\genpage

\section{Asymptotes}

\begin{snippetdefinition}{vertical-asymptote-definition}{Vertical asymptote}
    The line \(x=a\) is a \emph{vertical asymptote} of a \function \(f(x)\) is at least one of the following is true:
    \begin{enumerate}
        \item \(f\colon (\xi, a) \fromto \realnumbers\) for \(\xi \in \extendedrealnumbers\) and
            \[
                \lim_{x\to a^-}f(x) = \pm \infty
            \]
        \item \(f\colon (a, \xi) \fromto \realnumbers\) for \(\xi \in \extendedrealnumbers\) and
            \[
                \lim_{x\to a^+}f(x) = \pm \infty
            \]
    \end{enumerate}
\end{snippetdefinition}

\begin{snippetdefinition}{horizontal-asymptote-definition}{Horizontal asymptote}
    The line \(y=c\) is a \emph{horizontal asymptote} of a
    \function \(f\colon (a, +\infty) \fromto \realnumbers\)
    if
    \[
        \lim_{x\to\infty} f(x) = c
    \]
    or \(f\colon (-\infty, a) \fromto \realnumbers\)
    if
    \[
        \lim_{x\to-\infty} f(x) = c
    \]
\end{snippetdefinition}

\begin{snippetdefinition}{oblique-asymptote-definition}{Oblique asymptote}
    The line \(y=mx+q\) is a \emph{horizontal asymptote} of a
    \function \(f\colon (a, +\infty) \fromto \realnumbers\)
    if
    \[
        \lim_{x\to\infty} f(x) - mx = q
    \]
    or \(f\colon (-\infty, a) \fromto \realnumbers\)
    if
    \[
        \lim_{x\to-\infty} f(x) - mx = q
    \]
\end{snippetdefinition}

\begin{snippettheorem}{convex-function-asymptote-theorem}{}
    Let \(f\colon (a, +\infty) \fromto \realnumbers\) be a \function that is convex in \((a, +\infty)\).
    If \(y = mx + q\) is an asymptote for \(x\to +\infty\), then \[\forall x \in (a,+\infty), f(x) \geq mx+q\]
\end{snippettheorem}

\plain{Likewise, it is always under if the function is concave.}
% E anche per la dis. stretta.

\begin{snippetproof}{convex-function-asymptote-theorem-proof}{convex-function-asymptote-theorem}{}
    \todo
\end{snippetproof}

\end{document}