\documentclass[preview]{standalone}

\usepackage{amsmath}
\usepackage{amssymb}
\usepackage{stellar}
\usepackage{definitions}

\begin{document}

\id{complexanalysis-trigonometric-form}
\genpage

\section{Trigonometric form}

\begin{snippettheorem}{complex-number-trig-form}{Complex Number Trigonometric Form}
    Any complex number \(z=a+bi\) can be represented in a trigonometric form
    \[
        a+bi=r(\cos\theta+i\sin\theta)
    \]
    where \(r=|z|\) and \(\theta = \arg(z)\).
\end{snippettheorem}

\begin{snippetproposition}{product-of-complex-trig-forms}{Product of trigonometric forms}
    Let \(w = r(\cos\theta + i\sin\theta), z = \rho(\cos\varphi + i\sin\varphi)\) be complex numbers. Then,
    \[
        zw = r\rho \left[ \cos(\theta + \varphi) + i\sin(\theta + \varphi) \right]
    \]
\end{snippetproposition}

\begin{snippetproof}{product-of-complex-trig-forms-proof}{product-of-complex-trig-forms}{Product of trigonometric forms}
    Let \(w = r(\cos\theta + i\sin\theta), z = \rho(\cos\varphi + i\sin\varphi)\) be complex numbers. Then,
    \begin{align*}
        zw &= r\rho (\cos\theta + i\sin\theta)(\cos\varphi + i\sin\varphi) \\
        &= r\rho \left[ (\cos\theta\cos\varphi - \sin\theta\sin\varphi) + i(\sin\theta\cos\varphi + \cos\theta\sin\varphi) \right] \\
        &= r\rho \left[ \cos(\theta + \varphi) + i\sin(\theta + \varphi) \right]
    \end{align*}
\end{snippetproof}

\begin{snippetproposition}{inverse-of-complex-trig-form}{Inverse of complex trigonometric form}
    Let \(z = r(\cos\theta + i\sin\theta)\) be a complex number where \(r>0\). Then,
    \[
        z^{-1} = \frac{1}{r}(\cos(-\theta) + i\sin(-\theta))
    \]
\end{snippetproposition}

\end{document}