\documentclass[preview]{standalone}

\usepackage{amsmath}
\usepackage{amssymb}
\usepackage{stellar}
\usepackage{definitions}

\begin{document}

\id{mechanics-conservative-forces}
\genpage

\section{Conservative forces}

\begin{snippetdefinition}{conservative-force-definition}{Conservative force}
    A \emph{conservative force} is a positional force such that
    \[
        \vec{F}(\vec{r}) = -\gradient U(\vec{r})
    \]
\end{snippetdefinition}

\plain{Not all positional forces are conservative; the gradient condition must be satisfied.}

\begin{snippettheorem}{work-of-a-conservative-force-theorem}{Work of a conservative force}
    Consider a body only subject to conservative forces \(\vec{F}(\vec{r})\). Then,
    \[
        W = U(A) - U(B)
    \]
\end{snippettheorem}

\begin{snippetproof}{work-of-a-conservative-force-theorem-proof}{work-of-a-conservative-force-theorem}{Work of a conservative force}
    Consider the work
    \begin{align*}
        W &= \sum_{i=1}^N \vec{F_i} \cdot \Delta \vec{s_i} \\
        &= \sum_{i=1}^N \vec{F_i} \cdot |\Delta \vec{s_i}| \frac{\Delta \vec{s_i}}{|\Delta \vec{s_i}|}
    \end{align*}
    The last term is a directional vector, and thus we have the directional derivative
    \begin{align*}
        W &= \int_C \vec{F} \,d\vec{s} \\
        &= - \sum_{i=1}^N \left(
            \gradient U_i \cdot \vec{m_i}
        \right) |\Delta \vec{s_i}| \\
        &= - \sum_{i=1}^N \frac{
            U(\vec{r_{i-1}} + \Delta \vec{s_i}) - (\vec{r_{i-1}})
        }{
            |\Delta \vec{s_i}|
        } |\Delta \vec{s_i}| \\
        &= - \left[
            U(\vec{r_1}) - U(\vec{r_0}) + U(\vec{r_2}) - U(\vec{r_1})
            + \cdots + U(\vec{r_N}) - U(\vec{r_{N-1}})
        \right] \\
        &= U(\vec{r_0}) - U(\vec{r_N}) \\
        &= U(A) - U(B)
    \end{align*}
\end{snippetproof}

\subsection{Energy conservation}

\plain{By putting together this theorem and the work-energy theorem, we get the mechanical energy conservation.}

\begin{snippettheorem}{mechanical-energy-conservation-theorem-theorem}{Mechanical energy conservation theorem}
    For any conservative force,
    \[
        E_C(A) + U(A) = E_C(B) + U(B)
    \]
\end{snippettheorem}

\section{Examples}

\begin{snippetproposition}{weight-force-potential-energy}{Weight force potential energy}
    Consider the weight force \(F_z = -mg = -\gradient U\). Then,
    \[
        U(z) = mgz
    \]
\end{snippetproposition}

\begin{snippetproposition}{elastic-force-potential-energy}{Elastic force potential energy}
    Consider the elastic force \(F_x = -kx = -\gradient U\). Then,
    \[
        U(z) = \frac{1}{2}kx^2
    \]
\end{snippetproposition}

\end{document}