\documentclass[preview]{standalone}

\usepackage{amsmath}
\usepackage{amssymb}
\usepackage{stellar}
\usepackage{definitions}

\begin{document}

\id{arbitrary-particle-motion}
\genpage

\section{Arbitrary motion}

\begin{snippettheorem}{arbitrary-particle-motion-theorem}{Arbitrary particle motion}
    Let \(\vec{r}(t)\) be an arbitrary vector representing the motion of a particle.
    Then, its acceleration has tangential component and a normal component (\emph{centripetal} component)
    \[
        \vec{a}(t) = \frac{dv(t)}{dt}\vec{T} + \frac{v^2}{R}\vec{N}
    \]
    where \(v\) is the velocity and \(R\) is the \emph{radius of curvature}.
\end{snippettheorem}

\begin{snippetproof}{arbitrary-particle-motion-theorem-proof}{arbitrary-particle-motion-theorem}{Arbitrary particle motion}
    The velocity is given by \(\vec{v}(t) = \frac{d\vec{r}(t)}{dt}\) which is a vector pointing in the direction of the trajectory.
    The tangent vector is defined such that
    \[
        \hat{T}(t) v(t) = \vec{v}(t)
    \]
    And thus we have
    \[
        \vec{a}(t) = \frac{d}{dt} \left(v(t)\hat{T}(t)\right) = \frac{dv(t)}{dt}\hat{T}(t) + v(t)\frac{d\hat{T}(t)}{dt} = a(t)\hat{T}(t) + v(t)\frac{d\hat{T}(t)}{dt}
    \]
    In order to study the meaning of such terms, we start by the identity \(\hat{T}(t) \cdot \hat{T}(t) = 1\).
    Then,
    \begin{align*}
        \frac{d}{dt} \left( \hat{T}(t) \cdot \hat{T}(t) \right) &= 0 \\
        \frac{d\hat{T}(t)}{dt} \cdot \hat{T}(t) + \hat{T}(t)\frac{d\hat{T}(t)}{dt} &= 0 \\
        \hat{T}(t)\frac{d\hat{T}(t)}{dt} &= 0 
    \end{align*}
    which means that \(\frac{d\hat{T}(t)}{dt}\) and \(\hat{T}(t)\) are orthogonal.
    Indeed,
    \[
        \frac{d\hat{T}(t)}{ds} = \hat{N}
    \]
    By the differential analysis we find
    \[
        \left|\frac{d\hat{T}(t)}{dt}\right| = \lim_{\Delta t \to 0} \frac{ds}{\Delta t}
    \]
    where \(ds\) is the length of the space traversed. In the limite,
    this length if the circular arc of radius \(R\), where \(R\) is the length of the line to the rotation point (radius of curvature, meaning the radius of the osculating circle).
    Thus,
    and the circular arc
    \[
        ds = Rd\theta
    \]
    which also means that \(d\theta = \frac{ds}{R}\).
    By putting together these two information we find
    \[
        \left|\frac{d\hat{T}(t)}{dt}\right| = \lim_{\Delta t \to 0} \left[\frac{ds}{\Delta t} \frac{1}{R}\right] = \frac{v}{R}
    \]
    and now we can write
    \[
        \vec{a}(t) = \frac{dv}{dt}\hat{T} + v\frac{d\hat{T}}{dt} = \frac{dv}{dt}\hat{T} + \frac{v^2}{R} \hat{N}
    \]
\end{snippetproof}

\plain{Note that the centripetal acceleration is smaller the bigger the circle is, and thus null when the particle is
moving on a straight line.}

\subsection{Circular motion}

\begin{snippetproposition}{uniform-circular-motion}{Uniform circular motion}
    A uniform circular motion only has a centripetal acceleration
    \[
        \vec{a} = -\omega^2\vec{r} = \frac{v^2}{R} \hat{N}
    \]
    where \(\omega = \frac{v}{R}\).
\end{snippetproposition}

\end{document}