\documentclass[preview]{standalone}

\usepackage{amsmath}
\usepackage{amssymb}
\usepackage{stellar}
\usepackage{definitions}
\usepackage{bettelini}

\begin{document}

\id{metric-spaces-examples}
\genpage

\section{Examples}

\begin{snippetexample}{valley-metric-example}{Valley metric}
    The \textit{valley metric} \distancefunctiontext between the point
    \(a=(x,y)\) and \(b=(t,u)\) is defined as
    \[
        \distancefunction[d](a, b) = \begin{cases}
            |y-u| & x = t \\
            |y| + |x-t| + |u| & x \neq t
        \end{cases}
    \]
    which satisfies the conditions for the \distancefunctiontext:
    \begin{enumerate}
        \item \textbf{Nullity:} \\ \iffproof{
            If \(x=t\), \(\distancefunction[d](a,b) = 0 \implies \distancefunction[d](a,b) = |y-u|\).
            The term \(|y-u|\) is \(0\) \ifandonlyif \(y-u = 0\) \\
            and thus \(y=u\). Since \(x=t\), \(a=b\).
            Otherwise, \(\distancefunction[d](a,b) = 0 \implies |y| + |x-t| + |u| = 0\). \\
            This term is \(0\) \ifandonlyif \(|y| = 0 \land |x-t| = 0 \land |u| = 0\).
            Thus, \(x-t=0\implies x=t\). \\
            However, \(x\neq t\) \lightning, so this latter case is impossible.
        }{
            Let \(a = b\). Then, \(\distancefunction[d](a,b) = |y-u| = 0\).
        }
        \item \textbf{Positivity:} If \(x=t\), \(\distancefunction[d](a,b) = |y-u| \geq 0\).
            Otherwise, \(\distancefunction[d](a,b) = |y| + |x-t| + |u| \geq 0\).
        \item \textbf{Simmetry:} If \(x=t\), \(\distancefunction[d](a,b) = |y-u| = |u-y| = \distancefunction[d](b,a)\).
            Otherwise, \[\distancefunction[d](a,b) = |y| + |x-t| + |u| = |u| + |t-x| + |y| = \distancefunction[d](b,a) \]
        \item \textbf{Triangle inequality:} Let \(m = (m_x, m_y)\).
            Then, if \(x=t\) and \(m_x=m_y\), \[\distancefunction[d](a,b) = |y-u| \leq |y-m_y| + |m_y - u| = \distancefunction[d](a,m) + \distancefunction[d](m,b)\]
            Otherwise, \[\distancefunction[d](a,b) = |y| + |x-t| + |u| \leq |y| + |x-m_x| + |m_y| + |m_y| + |m_x-t| + |u| =\distancefunction[d](a,m) + \distancefunction[d](m,b)\]
    \end{enumerate}
\end{snippetexample}

\begin{snippetexample}{graph-distance-example}{Graph metric}
    Let \(G=(V,E)\) be a \graph. The \distancefunctiontext between two vertices \(a,b\in V\)
    is defined as
    \[
        \distancefunction[d](a, b) = \inf S
    \]
    where \(S\) is the \set of all \walk[walks] between \(a\) and \(b\).
\end{snippetexample}

\end{document}