\documentclass[preview]{standalone}

\usepackage{amsmath}
\usepackage{amssymb}
\usepackage{parskip}
\usepackage{fullpage}
\usepackage{hyperref}
\usepackage{bettelini}
\usepackage{stellar}

\hypersetup{
    colorlinks=true,
    linkcolor=black,
    urlcolor=blue,
    pdftitle={Zeta Function},
    pdfpagemode=FullScreen,
}

\begin{document}

\title{Zeta Function}
\id{zetafunction-definition}
\genpage

\plain{<br>}

\begin{snippetdefinition}{zeta-function-definition}{Zeta Function}
    The \textit{zeta function} is defined as
    \[
        \zeta(s)=\sum_{n=1}^{\infty}\frac{1}{n^s},\quad \Re(s)>1
    \]
\end{snippetdefinition}

\begin{snippettheorem}{zeta-function-euler-product}{Zeta function as Euler product}
    The zeta function can be represented as the Euler product
    \[
        \zeta(s)=\prod_{p\in P}^{\infty}\frac{1}{1-p^{-s}}
    \]
\end{snippettheorem}

\begin{snippetproof}{zeta-function-euler-product-proof}{Zeta function as Euler product}
    We start by using the first prime number: 2, and multiply both sides by \(2^{-s}\).
    \begin{align*}
        \zeta(s)\frac{1}{2^s}=\sum_{n=1}^{\infty}\frac{1}{{(2n)}^s}
    \end{align*}
    We then subtract the second definition from the first one, such that
    \begin{align*}
        \zeta(s)-\zeta(s)\frac{1}{2^s}&=
        \sum_{n=1}^{\infty}\left[\frac{1}{n^s}\right]-
        \sum_{n=1}^{\infty}\left[\frac{1}{{(2n)}^s}\right]
        \\
        \zeta(s)\left(1-\frac{1}{2^s}\right)&=
        \sum_{n=1}^{\infty}\frac{1}{n^s},
        \quad n\neq 2k,k\in \mathbb{Z}
    \end{align*}
    Here we are excluding the multiples of 2 from the series.
    
    If we do the same with the next prime number, which is 3, we get
    \begin{align*}
        \zeta(s)\left(1-\frac{1}{2^s}\right)\left(1-\frac{1}{3^s}\right)&=
        \sum_{n=1}^{\infty}\frac{1}{n^s},
        \quad n\neq 2k,n\neq 3k, k\in \mathbb{Z}
    \end{align*}
    
    We can repeat this process with every prime number.
    \\
    Eventually, we will exclude every nth-term to sum as we use every prime number, except for n=1.
    \begin{align*}
        \zeta(s)\prod_{p\in P}^{\infty}1-\frac{1}{p^s}=\frac{1}{1^s}=1
    \end{align*}
    Finally, we get the identity
    \begin{align*}
        \zeta(s)=
        \prod_{p\in P}^{\infty}\frac{1}{1-p^{-s}}
    \end{align*}
\end{snippetproof}

\end{document}
