\documentclass{article}
\usepackage[utf8]{inputenc}
\usepackage{amsmath}
\usepackage{amssymb}
\usepackage{parskip}
\usepackage{fullpage}
\usepackage{hyperref}
\usepackage{tikz}

\hypersetup{
    colorlinks=true,
    linkcolor=black,
    urlcolor=blue,
    pdftitle={Differentiation},
    pdfpagemode=FullScreen,
}

\title{Differentiation}
\author{Paolo Bettelini}
\date{}

\begin{document}

\maketitle
\tableofcontents
\pagebreak

\section{Definition}

\begin{center}
    \begin{tikzpicture}[scale=3]
        \draw[
            domain=-0.5:3,
            smooth,
            very thick,
            blue]
            plot ({\x}, {\x*sin(\x r)});
        \draw[gray, very thick] (0.75,0.5) -- node [below] {\(\Delta x\)} ++ (0.75,0);
        \draw[gray, very thick] (1.5,0.5) -- node [right] {\(\Delta y\)} ++ (0,1);
        \draw[gray, red] (0.375,0) -- (1.725,1.8);
    \end{tikzpicture}
\end{center}

\[
    \lim_{h \to 0^{+}} f(x)
    =\frac{f(x+h)-f(x)}{h}
\]

\pagebreak

\section{Chain Rule}

\subsection{Definition}

If \(z\) depends on \(y\), and \(y\) depends on \(x\), then \(z\) also depends on \(x\).

\[
    \frac{dz}{dx}=\frac{dz}{dy}\cdot\frac{dy}{dx}
\]

\subsection{Proof}

Assuming that \(z\) and \(y\) are differentiable in \(x\)

\begin{align*}
    \frac{dz}{dx}
    &= \lim_{\Delta x \to 0} \frac{\Delta z}{\Delta x}
    = \lim_{\Delta x \to 0} \frac{\Delta z}{\Delta y} \cdot \frac{\Delta y}{\Delta x} \\
    &= \left(
        \lim_{\Delta x \to 0} \frac{\Delta z}{\Delta y}
    \right)
    \left(
        \lim_{\Delta x \to 0} \frac{\Delta y}{\Delta x}
    \right) \\
    &= \left(
        \lim_{\Delta x \to 0} \frac{\Delta z}{\Delta y}
    \right)
    \cdot
    \frac{dy}{dx}
\end{align*}

As \(\Delta x \to 0\) also \(\Delta y \to 0\), so we can replace \(\Delta x\) with \(\Delta y\)

\begin{align*}
    \frac{dz}{dx}
    &= \left(
        \lim_{\Delta y \to 0} \frac{\Delta z}{\Delta y}
    \right)
    \cdot
    \frac{dy}{dx} \\
    &= \frac{dz}{dy} \cdot \frac{dy}{dx}
\end{align*}

\pagebreak

\section{Rules for differentiation}

\[
    \frac{d}{dx}(n)=0
\]

\[
    \frac{d}{dx}(x^n)=nx^{n-1},\quad n\in\mathbb{R}^*
\]

\[
    \frac{d}{dx}\left(n\cdot f(x)\right)=n\frac{d}{dx}\left(f(x)\right)
\]

\[
    \frac{d}{dx}(f+g)=f'+g'
\]

\[
    \frac{d}{dx}(f\cdot g)=g'f+gf'
\]

\[
    \frac{d}{dx}(f(g(x)))=f'(g(x))\cdot g'(x)
\]

\[
    \frac{d}{dx}(f^g)=f^g\left(\frac{f'g}{f}+g'\ln f\right)
\]

\end{document}
